ToCoq sans option ni check

ToCoq.v
@@ -1,9 +1,11 @@
-Require Import Defs Mix Proofs Meta Omega.
+Require Import Defs Mix Proofs Meta Omega Setoid Morphisms.
 Import ListNotations.
 Local Open Scope bool_scope.
 Local Open Scope lazy_bool_scope.
 Local Open Scope string_scope.
 Local Open Scope eqb_scope.
+
+Set Implicit Arguments.
 
 Fixpoint arity_fun A n B :=
   match n with
@@ -20,74 +22,86 @@ Definition get_arity {A B} (o : option { n:nat & arity_fun A n B}) :=
 Definition modfuns M := string -> option { n:nat & arity_fun M n M }.
 Definition modpreds M := string -> option { n:nat & arity_fun M n Prop }.
 
-Section SIGN.
+Record PreModel (M:Type)(sign:gen_signature) :=
+  { someone : M; (* M is non-empty *)
+    funs : modfuns M;
+    preds : modpreds M;
+    funsOk : forall s, sign.(gen_fun_symbs) s = get_arity (funs s);
+    predsOk : forall s, sign.(gen_pred_symbs) s = get_arity (preds s)
+  }.
+
+(** A premodel is also called a Σ-structure. For a complete model
+    of a theorie, we'll need the axioms of the theories, and
+    the facts that their interpretations are valid. *)
+
+(** Note: actually, we're not using [sign], [funsOk], [predsOK]
+    anywhere in this file (yet?) !! *)
+
+Section PREMODEL.
  Variable sign : gen_signature.
  Variable M:Type.
- Variable funs : modfuns M.
- Variable preds : modpreds M.
-
- Definition Adequate :=
-  (exists m:M, Logic.True) /\
-  (forall s, sign.(gen_fun_symbs) s = get_arity (funs s)) /\
-  (forall s, sign.(gen_pred_symbs) s = get_arity (preds s)).
-
-
-Definition optbind {A B} (o:option A)(f:A->option B) : option B :=
- match o with
- | None => None
- | Some x => f x
- end.
-
-Infix ">>=" := optbind (at level 60).
+ Variable Mo : PreModel M sign.
 
 Definition build_args {A B} :=
-  fix build n (l : list (option A)) : arity_fun A n B -> option B :=
+  fix build n (l : list A)(def:B) : arity_fun A n B -> B :=
     match n, l with
-    | 0, [] => fun f => Some f
-    | S n, Some a :: l => fun f => build n l (f a)
-    | _, _ => fun _ => None
+    | 0, [] => fun f => f
+    | S n, a :: l => fun f => build n l def (f a)
+    | _, _ => fun _ => def
     end.
 
-Definition eval_term genv lenv :=
-  fix eval t :=
+(** In case of ill-formed term (w.r.t. signature [sign]), we'll
+    use the arbitrary point [Mo.(someone)]. Same if we encounter
+    a local variable larger than the local environment *)
+Definition BogusPoint := Mo.(someone).
+
+Definition interp_term genv lenv :=
+  fix interp t :=
     match t with
-    | FVar x => Some (genv x)
-    | BVar n => nth_error lenv n
-    | Fun f args => funs f >>= (fun '(existT _ n f) =>
-                                  build_args n (List.map eval args) f)
+    | FVar x => genv x
+    | BVar n => nth n lenv BogusPoint
+    | Fun f args =>
+      match Mo.(funs) f with
+      | Some (existT _ n f) =>
+        build_args n (List.map interp args) BogusPoint f
+      | None => BogusPoint
+      end
     end.
 
-Definition eval_op o :=
+Definition interp_op o :=
  match o with
  | And => and
  | Or => or
  | Imp => (fun p q : Prop => p -> q)
  end.
 
-Definition eval_form genv :=
-  fix eval lenv f :=
+(** In case of ill-formed formula (w.r.t. signature [sign]), we'll
+    evaluate to the arbitrary proposition [False]. *)
+Definition BogusProp := Logic.False.
+
+Definition interp_form genv :=
+  fix interp lenv f :=
     match f with
     | True => Logic.True
     | False => Logic.False
-    | Not f => ~(eval lenv f)
-    | Op o f1 f2 => eval_op o (eval lenv f1) (eval lenv f2)
+    | Not f => ~(interp lenv f)
+    | Op o f1 f2 => interp_op o (interp lenv f1) (interp lenv f2)
     | Pred p args =>
-      let optp := preds p >>= fun '(existT _ n f) =>
-                  build_args n (List.map (eval_term genv lenv) args) f
-      in match optp with
-         | Some p => p
-         | None => Logic.False
-         end
-    | Quant All f => forall (m:M), eval (m::lenv) f
-    | Quant Ex f => exists (m:M), eval (m::lenv) f
+      match Mo.(preds) p with
+      | Some (existT _ n f) =>
+        build_args n (List.map (interp_term genv lenv) args) BogusProp f
+      | None => BogusProp
+      end
+    | Quant All f => forall (m:M), interp (m::lenv) f
+    | Quant Ex f => exists (m:M), interp (m::lenv) f
     end.
 
-Definition eval_ctx genv lenv l :=
-  forall f, In f l -> eval_form genv lenv f.
+Definition interp_ctx genv lenv l :=
+  forall f, In f l -> interp_form genv lenv f.
 
-Definition eval_seq genv lenv '(Γ⊢C) :=
-  eval_ctx genv lenv Γ ->
-  eval_form genv lenv C.
+Definition interp_seq genv lenv '(Γ⊢C) :=
+  interp_ctx genv lenv Γ ->
+  interp_form genv lenv C.
 
 Lemma max_0 n m : Nat.max n m = 0 <-> n=0 /\ m=0.
 Proof.
@@ -99,71 +113,28 @@ Proof.
  induction l; simpl; rewrite ?max_0 in *; intuition.
 Qed.
 
-Lemma build_args_uncheck {A B} n l (f:arity_fun A n B) :
-  List.length l <> n \/ In None l <-> build_args n l f = None.
-Proof.
- revert n l f.
- induction n; destruct l as [|o l]; cbn; intros f; auto.
- - intuition easy.
- - intuition easy.
- - intuition easy.
- - destruct o. rewrite <- IHn; intuition; easy. intuition.
-Qed.
-
-Lemma eval_term_notNone :
- Adequate ->
- forall genv (t:term),
- check sign t = true /\ closed t = true <->
-  eval_term genv [] t <> None.
-Proof.
- intros (_ & AD & _) genv.
- fix IH 1. destruct t; cbn; auto; try easy.
- - destruct n; cbn in *; intuition.
- - rewrite AD. destruct (funs f) as [(n,fn)|]; cbn; [|intuition].
-   case eqbspec; intro LN.
-   + clear f.
-     assert (E : build_args n (map (eval_term genv []) l) fn <> None
-             <-> ~In None (map (eval_term genv []) l)).
-     { rewrite <- build_args_uncheck, map_length. intuition. }
-     rewrite E; clear E.
-     clear n fn LN. rewrite eqb_eq. revert l.
-     fix IH' 1. destruct l; cbn; auto.
-     intuition.
-     rewrite andb_true_iff, max_0.
-     specialize (IH' l). specialize (IH t).
-     unfold closed in IH. rewrite eqb_eq in IH.
-     intuition.
-   + rewrite <- build_args_uncheck, map_length. intuition.
-Qed.
-
-Lemma eval_term_ext genv genv' lenv t :
+Lemma interp_term_ext genv genv' lenv t :
  (forall v, Vars.In v (fvars t) -> genv v = genv' v) ->
- eval_term genv lenv t = eval_term genv' lenv t.
+ interp_term genv lenv t = interp_term genv' lenv t.
 Proof.
  revert t.
  fix IH 1. destruct t; cbn; auto.
- - intros. f_equal. apply H. varsdec.
- - intros. case (funs f) as [(n,fn)|]; cbn; auto. clear f.
+ - intros. apply H. varsdec.
+ - intros. case (Mo.(funs) f) as [(n,fn)|]; cbn; auto. clear f.
    f_equal. clear n fn. revert l H.
    fix IH' 1. destruct l; cbn; auto.
    intros E. f_equal; auto with set.
 Qed.
 
-Lemma eval_form_ext genv genv' lenv f :
+Lemma interp_form_ext genv genv' lenv f :
  (forall v, Vars.In v (fvars f) -> genv v = genv' v) ->
- eval_form genv lenv f <-> eval_form genv' lenv f.
+ interp_form genv lenv f <-> interp_form genv' lenv f.
 Proof.
  revert lenv.
  induction f; cbn; auto; intros; f_equal; auto with set.
- - case (preds p) as [(n,fn)|]; cbn; [|reflexivity]; clear p.
-   assert (E : map (eval_term genv lenv) l =
-               map (eval_term genv' lenv) l).
-   { clear n fn.
-     revert l H.
-     induction l; cbn; auto.
-     intros E. f_equal; auto with set. apply eval_term_ext.
-     auto with set. }
-   now rewrite E.
+ - case (Mo.(preds) p) as [(n,fn)|]; cbn; [|reflexivity]; clear p.
+   f_equiv. clear n fn. revert l H. induction l; cbn; auto.
+   intros E. f_equal; auto using interp_term_ext with set.
  - rewrite IHf; intuition.
  - destruct o; cbn; rewrite IHf1, IHf2; intuition.
  - destruct q.
@@ -173,80 +144,85 @@ Proof.
      [rewrite <-IHf|rewrite IHf]; auto with set.
 Qed.
 
-Lemma eval_ctx_ext genv genv' lenv c :
+Lemma interp_ctx_ext genv genv' lenv c :
  (forall v, Vars.In v (fvars c) -> genv v = genv' v) ->
- eval_ctx genv lenv c <-> eval_ctx genv' lenv c.
+ interp_ctx genv lenv c <-> interp_ctx genv' lenv c.
 Proof.
  intros E.
- unfold eval_ctx.
+ unfold interp_ctx.
  split; intros H f Hf.
- rewrite <- (eval_form_ext genv); auto with set.
+ rewrite <- (interp_form_ext genv); auto with set.
  intros v Hv. apply E. unfold fvars, fvars_list.
  rewrite vars_unionmap_in. exists f. now split.
- rewrite (eval_form_ext genv); auto with set.
+ rewrite (interp_form_ext genv); auto with set.
  intros v Hv. apply E. unfold fvars, fvars_list.
  rewrite vars_unionmap_in. exists f. now split.
 Qed.
 
-Lemma eval_term_more_lenv genv lenv lenv' t :
- eval_term genv lenv t <> None ->
- eval_term genv (lenv++lenv') t = eval_term genv (lenv) t.
+Lemma interp_term_more_lenv genv lenv lenv' t :
+ (level t <= List.length lenv)%nat ->
+ interp_term genv (lenv++lenv') t = interp_term genv lenv t.
 Proof.
  revert t.
  fix IH 1. destruct t; cbn in *; intros H.
  - reflexivity.
- - rewrite nth_error_app1; trivial.
-   now apply nth_error_Some.
- - case (funs f) as [(k,fk)|]; cbn in *; auto.
+ - rewrite app_nth1; trivial.
+ - case (Mo.(funs) f) as [(k,fk)|]; cbn in *; auto.
    f_equal.
-   assert (H' : ~In None (map (eval_term genv lenv) l)).
-   { rewrite <- build_args_uncheck in H. intuition. }
-   clear H k fk f.
-   revert l H'.
+   clear k fk f.
+   revert l H.
    fix IH' 1. destruct l; cbn; auto.
-   intros H. f_equal; auto.
+   intros H. f_equal. apply IH. omega with *. apply IH'. omega with *.
 Qed.
 
-Lemma eval_term_bsubst genv lenv u m n t :
+Lemma interp_term_closed genv lenv t :
+ closed t = true ->
+ interp_term genv lenv t = interp_term genv [] t.
+Proof.
+ unfold closed. rewrite eqb_eq. intros E.
+ apply (interp_term_more_lenv genv [] lenv). simpl. omega.
+Qed.
+
+Lemma interp_term_bsubst genv lenv u m n t :
  (level t <= S n)%nat ->
- (List.length lenv = n) ->
- eval_term genv [] u = Some m ->
- eval_term genv (lenv++[m]) t = eval_term genv lenv (bsubst n u t).
+ List.length lenv = n ->
+ closed u = true ->
+ interp_term genv [] u = m ->
+ interp_term genv (lenv++[m]) t =
+  interp_term genv lenv (bsubst n u t).
 Proof.
  revert t.
- fix IH 1. destruct t; cbn; auto; intros LE Hn Hu.
+ fix IH 1. destruct t; cbn; auto; intros LE Hn CL Hu.
  - case eqbspec; intros.
-   + rewrite nth_error_app2; try omega.
-     replace (n0 - length lenv) with 0 by omega. simpl.
-     rewrite <- Hu. symmetry.
-     apply (eval_term_more_lenv genv [] lenv). now rewrite Hu.
-   + apply nth_error_app1. omega.
- - case (funs f) as [(k,fk)|]; cbn; auto. f_equal. clear f k fk.
-   revert l LE Hn.
+   + rewrite app_nth2; try omega.
+     replace (n0 - length lenv) with 0 by omega. cbn.
+     now rewrite interp_term_closed.
+   + apply app_nth1. omega.
+ - case (Mo.(funs) f) as [(k,fk)|]; cbn; auto. f_equal. clear f k fk.
+   revert l LE.
    fix IH' 1. destruct l; cbn; auto.
-   intros LE Hn. f_equal.
+   intros LE. f_equal.
    apply IH; auto. omega with *.
    apply IH'; auto. omega with *.
 Qed.
 
-Lemma eval_form_bsubst genv lenv u m n f :
+Lemma interp_form_bsubst genv lenv u m n f :
  (level f <= S n)%nat ->
- (List.length lenv = n) ->
- eval_term genv [] u = Some m ->
- eval_form genv (lenv++[m]) f <-> eval_form genv lenv (bsubst n u f).
+ List.length lenv = n ->
+ closed u = true ->
+ interp_term genv [] u = m ->
+ interp_form genv (lenv++[m]) f <-> interp_form genv lenv (bsubst n u f).
 Proof.
  revert n lenv.
  induction f; cbn; auto; intros; f_equal; auto with set.
- - case (preds p) as [(k,fk)|]; cbn; [|reflexivity]; clear p.
-   assert (E : map (eval_term genv (lenv++[m])) l =
-               map (eval_term genv lenv) (map (bsubst n u) l)).
-   { clear k fk.
-     revert l H H0.
-     induction l; cbn; auto.
-     intros LE E. f_equal.
-     apply eval_term_bsubst; auto. omega with *.
-     apply IHl; auto. omega with *. }
-   now rewrite E.
+ - case (Mo.(preds) p) as [(k,fk)|]; cbn; [|reflexivity]; clear p.
+   f_equiv.
+   clear k fk.
+   revert l H.
+   induction l; cbn; auto.
+   intros H. f_equal.
+   apply interp_term_bsubst; auto. omega with *.
+   apply IHl; auto. omega with *.
  - rewrite (IHf n); intuition.
  - destruct o; cbn; rewrite (IHf1 n), (IHf2 n); intuition; omega with *.
  - destruct q.
@@ -260,99 +236,100 @@ Proof.
        erewrite IHf; eauto with set. omega with *. simpl; auto.
 Qed.
 
-Lemma eval_form_bsubst0 genv u m f :
+Lemma interp_form_bsubst0 genv u m f :
  (level f <= 1)%nat ->
- eval_term genv [] u = Some m ->
- eval_form genv [m] f <-> eval_form genv [] (bsubst 0 u f).
+ closed u = true ->
+ interp_term genv [] u = m ->
+ interp_form genv [m] f <-> interp_form genv [] (bsubst 0 u f).
 Proof.
- intros LE.
- now apply (eval_form_bsubst genv [] u m 0 f).
+ intros. apply (@interp_form_bsubst genv [] u m 0 f); auto.
 Qed.
 
-Lemma eval_form_bsubst_adhoc genv m x f :
+Lemma interp_form_bsubst_adhoc genv m x f :
  (level f <= 1)%nat ->
  ~Vars.In x (fvars f) ->
- eval_form genv [m] f <->
- eval_form (fun v => if v =? x then m else genv v) []
+ interp_form genv [m] f <->
+ interp_form (fun v => if v =? x then m else genv v) []
   (bsubst 0 (FVar x) f).
 Proof.
  intros.
- rewrite <- eval_form_bsubst0 with (m:=m); auto.
- - apply eval_form_ext. intros v Hv.
+ rewrite <- interp_form_bsubst0 with (m:=m); auto.
+ - apply interp_form_ext. intros v Hv.
    case eqbspec; auto. intros ->. varsdec.
  - cbn. now rewrite eqb_refl.
 Qed.
 
-Definition eval_logic lg :=
+Definition CoqRequirements lg :=
  match lg with
  | Classic => forall A:Prop, A\/~A
  | Intuiti => Logic.True
  end.
 
+(** Note: we do not ask here for the derivation [d] to be
+    well-formed w.r.t. the signature [sign] (cf. [Mix.check]) !!
+    An ill-formed derivation will involve [BogusPoint] and/or
+    [BogusProp] in its evaluation. Since the derivation [d] is
+    valid, the ill-formed parts will cancel themselves during
+    the proof, as in [Pred("=",[])->Pred("=",[])], and we'll
+    end up with uninteresting (but true) evaluations. *)
+
 Lemma correctness :
- Adequate ->
  forall (d:derivation) logic genv,
- eval_logic logic ->
- check sign d = true ->
+ CoqRequirements logic ->
  closed d = true ->
  valid_deriv logic d = true ->
- eval_seq genv [] (dseq d).
+ interp_seq genv [] (dseq d).
 Proof.
- intros AD.
  induction d as [r s ds IH] using derivation_ind'.
  cbn - [valid_deriv_step].
  intros logic genv.
  rewrite !lazy_andb_iff. rewrite eqb_eq, !max_0.
- intros LG ((Cr,Cs),Cds) (Lr&Ls&Lds) (V,Vds).
- assert (IH' : Forall (fun d => forall genv, eval_seq genv [] (dseq d)) ds).
+ intros CR (Lr&Ls&Lds) (V,Vds).
+ assert (IH' : Forall (fun d => forall genv, interp_seq genv [] (dseq d)) ds).
  { rewrite Forall_forall, forallb_forall in *.
    rewrite list_max_0 in Lds.
    intros d Hd genv'. eapply IH; eauto.
    unfold closed. rewrite eqb_eq. apply Lds. now apply in_map. }
- clear IH Cds Vds. mytac; cbn in *; intros Hc.
+ clear IH Vds. cbn in *. break; mytac; cbn in *; intros Hc.
  - now apply Hc, list_mem_in.
- - destruct (H1 genv); auto.
- - intro Hf. apply (H1 genv).
+ - destruct (H genv); auto.
+ - intro Hf. apply (H genv).
    intros ? [<-|E]; auto.
- - apply (H6 genv); auto.
+ - apply (H4 genv); auto.
  - intuition.
  - apply (H genv); auto.
  - apply (H genv); auto.
  - intuition.
  - intuition.
- - destruct (H4 genv); auto.
-   + apply (H6 genv). intros ? [<-|E]; auto.
-   + apply (H5 genv). intros ? [<-|E]; auto.
- - intros Hf1. apply (H2 genv). intros ? [<-|E]; auto.
+ - destruct (H2 genv); auto.
+   + apply (H4 genv). intros ? [<-|E]; auto.
+   + apply (H3 genv). intros ? [<-|E]; auto.
+ - intros Hf1. apply (H genv). intros ? [<-|E]; auto.
  - apply (H1 genv); auto.
  - intros m.
    rewrite <- not_false_iff_true, negb_false_iff in H0.
    rewrite Vars.mem_spec in H0.
-   rewrite eval_form_bsubst_adhoc with (x:=v).
-   apply H4.
-   rewrite <- (eval_ctx_ext genv); auto.
+   rewrite interp_form_bsubst_adhoc with (x:=v).
+   apply H2.
+   rewrite <- (interp_ctx_ext genv); auto.
    intros y Hy. case eqbspec; auto. intros <-. varsdec.
    omega with *.
    varsdec.
- - assert (Hwit := eval_term_notNone AD genv wit).
-   destruct (eval_term genv [] wit) as [m|] eqn:E.
-   + rewrite <- eval_form_bsubst0 with (m:=m); auto.
-     rewrite !max_0 in Lds. intuition.
-   + unfold closed in Hwit. rewrite eqb_eq in Hwit. intuition.
- - assert (Hwit := eval_term_notNone AD genv wit).
-   destruct (eval_term genv [] wit) as [m|] eqn:E.
-   + exists m.
-     rewrite eval_form_bsubst0 with (u:=wit); auto.
-     rewrite !max_0 in Ls. intuition.
-   + unfold closed in Hwit. rewrite eqb_eq in Hwit. intuition.
+ - rewrite <- interp_form_bsubst0 with (u:=wit); auto.
+   rewrite !max_0 in Lds. intuition.
+   unfold closed. rewrite eqb_eq. intuition.
+ - exists (interp_term genv [] wit).
+   rewrite interp_form_bsubst0 with (u:=wit); auto.
+   rewrite !max_0 in Ls. intuition.
+   unfold closed. rewrite eqb_eq. intuition.
  - destruct (H3 genv) as (m & Hm); auto.
    rewrite <- not_false_iff_true, negb_false_iff in H0.
    rewrite Vars.mem_spec in H0.
-   rewrite eval_form_bsubst_adhoc with (x:=v) in Hm.
-   erewrite eval_form_ext.
+   rewrite interp_form_bsubst_adhoc with (x:=v) in Hm.
+   erewrite interp_form_ext.
    eapply H5.
    intros A [<-|HA]. eapply Hm.
-   rewrite <- (eval_form_ext genv); auto.
+   rewrite <- (interp_form_ext genv); auto.
    intros y Hy. case eqbspec; auto. intros ->.
    assert (Vars.In v (fvars c)).
    { unfold fvars, fvars_list. rewrite vars_unionmap_in.
@@ -361,25 +338,23 @@ Proof.
    intros y Hy. cbn. case eqbspec; auto. intros ->. varsdec.
    rewrite !max_0 in Lds. intuition.
    varsdec.
- - destruct (LG (eval_form genv [] f0)); auto.
+ - destruct (CR (interp_form genv [] f0)); auto.
    destruct (H genv). intros A [<-|HA]; auto.
 Qed.
 
-Lemma coherence :
- Adequate ->
- forall (d:derivation) logic,
- eval_logic logic ->
- check sign d = true ->
+(** We hence cannot have a valid proof of False in an empty context. *)
+
+Lemma coherence logic : CoqRequirements logic ->
+ forall (d:derivation),
  closed d = true ->
  valid_deriv logic d = true ->
  dseq d <> ([]⊢False)%form.
 Proof.
- intros AD d logic LG CH CL VD E.
- case AD. intros (m,_) _.
- set (genv := fun (_:variable) => m).
- assert (eval_seq genv [] (dseq d)).
+ intros CR d CL VD E.
+ set (genv := fun (_:variable) => Mo.(someone)).
+ assert (interp_seq genv [] (dseq d)).
  { apply correctness with logic; auto. }
  rewrite E in H. cbn in *. apply H. intros A. destruct 1.
 Qed.
 
-End SIGN.
+End PREMODEL.
